\documentclass{beamer}

\begin{document}

\title{solve : 2y'''-6y''+6y'-2=2x^{\frac12}e^x\\[5]\small {y(0)=1,y'(0)=2,y''(0)=1}}



\begin{frame}

\titlepage  
\end{frame}


\begin{frame}{variation of parameter}

\[
2y'''-6y''+6y'-2=2x^{\frac12}e^x \Rightarrow y'''-3y''+3y'-1=x^{\frac12}e^x
\]
\\[8]
characteristic equation:
\[
(\lambda-1)^3=0 \Rightarrow \lambda=1,1,1    
\]

\[
y_h=Ax^2e^{x}+Bxe^x+Ce^x
\]
\end{frame}

\begin{frame}{variation of parameter}
initial assumption
\[
 \left\{\begin{matrix}
        &u_1'y_1+u_2'y_2&=&0\\
        &u_1'y_1'+u_2'y_2'&=&f(x)\\
       \end{matrix}
 \right.

\]
promote to 3
\[\Rightarrow
 \left\{\begin{matrix}
        &u_1'y_1+u_2'y_2+u_3'y_3&=&0\\
        &u_1'y_1'+u_2'y_2'+u_3'y_3'&=&0\\
        &u_1'y_1''+u_2'y_2''+u_3'y_3''&=&f(x)\\
       \end{matrix}
 \right.

\]
\end{frame}
\begin{frame}
\scriptsize{u_1=\int \frac{\begin{bmatrix}
0&xe^x&(x^2)e^x&\\
0&(1+x)e^x&(2x+x^2)e^x&\\
x^{\frac12}e^x&(2+x)e^x&(2+4x+x^2)e^x&\\
\end{bmatrix}}{\begin{bmatrix}
e^x&xe^x&(x^2)e^x&\\
e^x&(1+x)e^x&2(2x+x^2)e^x&\\
e^x&(2+x)e^x&(2+4x+x^2)e^x&\\
\end{bmatrix}}dx
=\int \frac{\begin{bmatrix}
0&x&x^2&\\
0&1&2x&\\
x^{\frac12}&2&2+4x&\\
\end{bmatrix}}{\begin{bmatrix}
1&x&x^2&\\
0&1&2x&\\
0&2&2+4x&\\
\end{bmatrix}}dx

\\[5]=\int \frac{x^{\frac52}}{\begin{bmatrix}
1&x&x^2&\\
0&1&2x&\\
0&0&2&\\
\end{bmatrix}}dx=\int \frac{x^{\frac52}}{2}dx=\frac17x^{\frac72}}
\\[5]
\scriptsize{u_2=\int \frac{\begin{bmatrix}
1&0&x^2&\\
1&0&2x+x^2&\\
1&x^{\frac12}&2+4x+x^2&\\
\end{bmatrix}}{2}dx=\int \frac{-2x^{\frac32}}{2}dx=-\frac25x^{\frac52}}
\\[8]
\scriptsize{u_3=\int \frac{\begin{bmatrix}
1&x&0&\\
1&1+x&0&\\
1&2+x&x^{\frac12}&\\
\end{bmatrix}}{2}dx=\int \frac{x^{\frac12}}{2}dx=\frac13x^{\frac32}}

\end{frame}
\begin{frame}{variation of parameter}
\[y_p=y_1u_1+y_2u_2+y_3u_3=(\frac17-\frac25+\frac13)x^{\frac72}e^x\]
\[\Rightarrow  y=y_h+y_p=Ax^2e^{x}+Bxe^x+Ce^x+(\frac17-\frac25+\frac13)x^{\frac72}e^x\]


\[
 \left\{\begin{matrix}
        y(0)&=1&=&C&\\
        y'(0)&=2&=&B+C&\\
        y''(0)&=1&=&2A+2B+C&\\
       \end{matrix}
 \right.
\Rightarrow A=-1,B=1,C=1
\]
\[y=y_h+y_p=-x^2e^{x}+xe^x+e^x+\frac8{105}x^{\frac72}e^x\]
\end{frame}
\begin{frame}{method of convolution}
initial formula
\scriptsize{\[y=y_k(t)+y_s*f(t)=\mathcal{L}^{-1}\{\frac{(as+b)Y_0+aY_1}{as^2+bs+c}\}+\mathcal{L}^{-1}\{\frac{F(s)}{as^2+bs+c}\}\]
\normalsize{promote to 3}  
\scriptsize{\[\Rightarrow\mathcal{L}^{-1}\{\frac{(as^2+bs+c)Y_0+(as+b)Y_1+aY_2}{as^3+bs^2+cs+d}\}+\mathcal{L}^{-1}\{\frac{F(s)}{as^3+bs^2+cs+d}\}\]}}
\end{frame}

\begin{frame}{method of convolution}
    a=1, b=-3,c=3,d=-1
\[\Rightarrow y_s=\mathcal{L}^{-1}\{\frac{1}{(s-1)^3}\}=\frac{e^xx^2}2\]
\[y_s*f(x)=\int^x_0\frac{e^{x-t}(x-t)^2}2t^{\frac12}e^tdt=\frac{e^x}{2}\int^x_0x^2t^{\frac12}-2xt^{\frac32}+x^{\frac52}dt\]
\\[5]
\[=\frac{e^x}{2}[\frac23x^{\frac72}-\frac45x^{\frac72}+\frac27x^{\frac72}]=\frac8{105}x^{\frac72}e^x\]
\end{frame}


\begin{frame}{method of convolution}
    \[y_k=\mathcal{L}^{-1}\{\frac{(s^2-3s+3)(1)+(s-3)(2)+(1)}{(s-1)^3}\}=\mathcal{L}^{-1}\{\frac{(s^2-s-2)}{(s-1)^3}\}\\[5]=\mathcal{L}^{-1}\{\frac{-2}{(s-1)^3}+\frac1{(s-1)^2}+\frac1{s-1}\}=-x^2e^x+xe^x+e^x\]
\[y=y_s*f(x)+y_k=-x^2e^x+xe^x+e^x+\frac8{105}x^{\frac72}e^x\]
\end{frame}

\begin{frame}{class outline}
      
      \textbf{ First-order Differential Equations}
      
        \[\bullet Separable\;Equations\]
        \[\bullet Linear\;Equations\]
        \[\bullet Exact\;Equations\]
        \[\bullet Bernoulli\; Equations\]
      
        \textbf{Second-order Differential Equations}
      \[\bullet Homogeneous\; Solution\]
      \[\bullet Particular\;  Solution\]
        \[\bullet Variation \; Of\;  Parameter\]
        \textbf{Laplace Transform}
      \[\bullet Transform \;And \;Inverse \;Transform\]
        \[\bullet Method\; Of \;Convolution\]
    
\end{frame}
\begin{frame}{First-order Differential Equations }
     
        Separable Equations
        \[y'=\frac{f(x)}{g(y)}\Rightarrow \int g(y)dy=\int f(x)dx\]
        Linear Equations
        \[y'+p(x)y=g(x),let \;u(x)=e^{\int p(x)dx}\]
        Exact Equations
        \[M(x,y)dx+N(x,y)dy=0\]
        Bernoulli Equations
        \[y'+p(x)y=q(x)y^n ,let \;u(x)=y^{1-n}\]
     % Homogeneous Equations y=ux
     % riccati 帶入解答
      
\end{frame}

\begin{frame}{Second-order Differential Equations}
     
        homogeneous solution:
        \[a_k\lambda^k+a_{k-1}\lambda^{k-1}\cdots \]
        \[1.repeat \; root : A_{k-1}x^{k-1}e^{ax}+A_{k-2}x^{k-2}e^{ax}\cdots\]
        \[2.imagnary\; root: e^{(a+bi)x}\Rightarrow e^{ax}(A\cos(bx)+iB\sin(bx)) \] 
        \[3.other : Ae^{ax}+Be^{bx}\]
        particular solution
        \[e^x,\sin(x),\cos(x)\]
        variation of parameter
        
     
      
\end{frame}

\begin{frame}{Laplace Transform}
     
    Transform and inverse Transform
    \small{\[F(s)={\int^\infty_0} f(t)e^{-st}dt\]
    \[t^k\Rightarrow\frac{k!}{s^{k+1}}\]
    \[e^{at} \Rightarrow F(s)\rightarrow F(s-a)  \]
    \[e^{it}=\cos(t)+i\sin(t)\Rightarrow\frac{as+bi}{1+s^2}\]
    \[f^{(n)}(t)\Rightarrow s^nF(s)-s^{(n-1)}f(0)-s^{(n-2)}f'(0)\cdots\]
    \[\delta(t-t_0) \Rightarrow  e^{-st_0}\]
    \[u(t-a)=\frac{e^{-as}}{s}\]}
    method  of convolution
    
    
     
      
\end{frame}
\begin{frame}{my favorite part}
 \huge{laplace transform}
\end{frame}
\end{document}
